Red.v
@@ -1,0 +1,148 @@
+Require Import Misc.
+Require Import List.
+Require Import Freevar.
+Require Import Term.
+Require Import FEnv.
+
+Inductive nfval :=
+| NFFreeVar : freevar -> nfval
+| NFStructApp : nfval -> nfval_or_lam -> nfval
+
+with nfval_or_lam :=
+| NFVal : nfval -> nfval_or_lam
+| NFLam : freevar -> nfval_or_lam -> nfval_or_lam.
+
+Inductive envitem :=
+| EVal : nfval -> envitem
+| ELazy : term -> envitem
+| ELam : term -> freevar -> envitem.
+
+Inductive cont :=
+| KNil : cont
+| KUpdateLazy : freevar -> list term -> cont -> cont
+| KUpdateLam : term -> freevar -> cont -> cont
+| KApp : nfval -> list term -> cont -> cont.
+
+Record state := mkState {
+  st_code : envitem ;
+  st_stack : list term ;
+  st_env : list (freevar * envitem) ;
+  st_cont : cont ;
+  st_lamnf : list (freevar * nfval_or_lam) ;
+  st_usedvars : list freevar ;
+}.
+
+Inductive red : state -> state -> Prop :=
+| red_app : forall t u e pi K W L,
+    red {| st_code := ELazy (app t u) ; st_stack := pi ; st_env := e ; st_cont := K ; st_lamnf := W ; st_usedvars := L |}
+        {| st_code := ELazy t ; st_stack := u :: pi ; st_env := e ; st_cont := K ; st_lamnf := W ; st_usedvars := L |}
+| red_lam : forall t e pi K W L y,
+    y \notin L ->
+    red {| st_code := ELazy (lam t) ; st_stack := pi ; st_env := e ; st_cont := K ; st_lamnf := W ; st_usedvars := L |}
+        {| st_code := ELam t y ; st_stack := pi ; st_env := e ; st_cont := K ; st_lamnf := W ; st_usedvars := y :: L |}
+| red_redex : forall t u e pi K W L x y,
+    x \notin L ->
+    red {| st_code := ELam t y ; st_stack := u :: pi ; st_env := e ; st_cont := K ; st_lamnf := W ; st_usedvars := L |}
+        {| st_code := ELazy (t ^ x) ; st_stack := pi ; st_env := (x, ELazy u) :: e ; st_cont := K ; st_lamnf := W ; st_usedvars := x :: L |}
+| red_var_open : forall x e pi K W L,
+    env_find e x = None ->
+    red {| st_code := ELazy (fvar x) ; st_stack := pi ; st_env := e ; st_cont := K ; st_lamnf := W ; st_usedvars := L |}
+        {| st_code := EVal (NFFreeVar x) ; st_stack := pi ; st_env := e ; st_cont := K ; st_lamnf := W ; st_usedvars := L |}
+| red_var_val : forall x e v pi K W L,
+    env_find e x = Some (EVal v) ->
+    red {| st_code := ELazy (fvar x) ; st_stack := pi ; st_env := e ; st_cont := K ; st_lamnf := W ; st_usedvars := L |}
+        {| st_code := EVal v ; st_stack := pi ; st_env := e ; st_cont := K ; st_lamnf := W ; st_usedvars := L |}
+| red_var_lazy : forall x e t pi K W L,
+    env_find e x = Some (ELazy t) ->
+    red {| st_code := ELazy (fvar x) ; st_stack := pi ; st_env := e ; st_cont := K ; st_lamnf := W ; st_usedvars := L |}
+        {| st_code := ELazy t ; st_stack := nil ; st_env := e ; st_cont := KUpdateLazy x pi K ; st_lamnf := W ; st_usedvars := L |}
+| red_var_lam : forall x e t y pi K W L,
+    env_find e x = Some (ELam t y) ->
+    red {| st_code := ELazy (fvar x) ; st_stack := pi ; st_env := e ; st_cont := K ; st_lamnf := W ; st_usedvars := L |}
+        {| st_code := ELam t y ; st_stack := pi ; st_env := e ; st_cont := K ; st_lamnf := W ; st_usedvars := L |}
+| red_app_val : forall v e u pi K W L,
+    red {| st_code := EVal v ; st_stack := u :: pi ; st_env := e ; st_cont := K ; st_lamnf := W ; st_usedvars := L |}
+        {| st_code := ELazy u ; st_stack := nil ; st_env := e ; st_cont := KApp v pi K ; st_lamnf := W ; st_usedvars := L |}
+| red_lam_deepen : forall t x e K W L,
+    env_find W x = None ->
+    red {| st_code := ELam t x ; st_stack := nil ; st_env := e ; st_cont := K ; st_lamnf := W ; st_usedvars := L |}
+        {| st_code := ELazy (t ^ x) ; st_stack := nil ; st_env := e ; st_cont := KUpdateLam t x K ; st_lamnf := W ; st_usedvars := L |}
+| red_cont_app_val : forall v1 v2 pi K e W L,
+    red {| st_code := EVal v1 ; st_stack := nil ; st_env := e ; st_cont := KApp v2 pi K ; st_lamnf := W ; st_usedvars := L |}
+        {| st_code := EVal (NFStructApp v2 (NFVal v1)) ; st_stack := pi ; st_env := e ; st_cont := K ; st_lamnf := W ; st_usedvars := L |}
+| red_cont_app_lam : forall t x body v pi K e W L,
+    env_find W x = Some body ->
+    red {| st_code := ELam t x ; st_stack := nil ; st_env := e ; st_cont := KApp v pi K ; st_lamnf := W ; st_usedvars := L |}
+        {| st_code := EVal (NFStructApp v (NFLam x body)) ; st_stack := pi ; st_env := e ; st_cont := K ; st_lamnf := W ; st_usedvars := L |}
+| red_cont_update_lam_val : forall t v x K e W L,
+    red {| st_code := EVal v ; st_stack := nil ; st_env := e ; st_cont := KUpdateLam t x K ; st_lamnf := W ; st_usedvars := L |}
+        {| st_code := ELam t x ; st_stack := nil ; st_env := e ; st_cont := K ; st_lamnf := (x, NFVal v) :: W ; st_usedvars := L |}
+| red_cont_update_lam_lam : forall t1 t2 y body x K e W L,
+    env_find W y = Some body ->
+    red {| st_code := ELam t2 y ; st_stack := nil ; st_env := e ; st_cont := KUpdateLam t1 x K ; st_lamnf := W ; st_usedvars := L |}
+        {| st_code := ELam t1 x ; st_stack := nil ; st_env := e ; st_cont := K ; st_lamnf := (x, NFLam y body) :: W ; st_usedvars := L |}
+| red_cont_update_lazy_val : forall v x pi e K W L,
+    red {| st_code := EVal v ; st_stack := nil ; st_env := e ; st_cont := KUpdateLazy x pi K ; st_lamnf := W ; st_usedvars := L |}
+        {| st_code := EVal v ; st_stack := pi ; st_env := update_env e x (EVal v) ; st_cont := K ; st_lamnf := W ; st_usedvars := L |}
+| red_cont_update_lazy_lam : forall t y x pi e K W L,
+    red {| st_code := ELam t y ; st_stack := nil ; st_env := e ; st_cont := KUpdateLazy x pi K ; st_lamnf := W ; st_usedvars := L |}
+        {| st_code := ELam t y ; st_stack := pi ; st_env := update_env e x (ELam t y) ; st_cont := K ; st_lamnf := W ; st_usedvars := L |}
+.
+
+Fixpoint read_nfval (v : nfval) :=
+  match v with
+  | NFFreeVar x => fvar x
+  | NFStructApp v1 v2 => app (read_nfval v1) (read_nfval_or_lam v2)
+  end
+
+with read_nfval_or_lam (v : nfval_or_lam) :=
+  match v with
+  | NFVal v => read_nfval v
+  | NFLam x v => lam (closeb 0 x (read_nfval_or_lam v))
+  end.
+
+Definition read_envitem (ei : envitem) :=
+  match ei with
+  | EVal v => read_nfval v
+  | ELam t x => lam t
+  | ELazy t => t
+  end.
+
+Fixpoint read_stack t pi :=
+  match pi with
+  | nil => t
+  | u :: pi => read_stack (app t u) pi
+  end.
+
+
+Fixpoint nfval_ind2 (P : nfval -> Prop) (Q : nfval_or_lam -> Prop)
+         (Hfree : forall x, P (NFFreeVar x)) (Happ : forall v1 v2, P v1 -> Q v2 -> P (NFStructApp v1 v2))
+         (Hval : forall v, P v -> Q (NFVal v)) (Hlam : forall x v, Q v -> Q (NFLam x v)) v : P v :=
+  match v with
+  | NFFreeVar x => Hfree x
+  | NFStructApp v1 v2 => Happ v1 v2 (nfval_ind2 P Q Hfree Happ Hval Hlam v1) (nfval_or_lam_ind2 P Q Hfree Happ Hval Hlam v2)
+  end
+
+with nfval_or_lam_ind2 (P : nfval -> Prop) (Q : nfval_or_lam -> Prop)
+         (Hfree : forall x, P (NFFreeVar x)) (Happ : forall v1 v2, P v1 -> Q v2 -> P (NFStructApp v1 v2))
+         (Hval : forall v, P v -> Q (NFVal v)) (Hlam : forall x v, Q v -> Q (NFLam x v)) v : Q v :=
+  match v with
+  | NFVal v => Hval v (nfval_ind2 P Q Hfree Happ Hval Hlam v)
+  | NFLam x v => Hlam x v (nfval_or_lam_ind2 P Q Hfree Happ Hval Hlam v)
+  end.
+
+Definition nfval_and_lam_ind2 P Q Hfree Happ Hval Hlam :=
+  conj (fun v => nfval_ind2 P Q Hfree Happ Hval Hlam v) (fun v => nfval_or_lam_ind2 P Q Hfree Happ Hval Hlam v).
+
+
+Lemma nfval_and_lam_lc :
+  (forall v, lc (read_nfval v)) /\ (forall v, lc (read_nfval_or_lam v)).
+Proof.
+  apply nfval_and_lam_ind2.
+  - intros; simpl; constructor.
+  - intros; simpl; constructor; assumption.
+  - intros; simpl; assumption.
+  - intros; simpl. apply lc_lam_body. apply closeb_body. assumption.
+Qed.
+
+Definition nfval_or_lam_lc := proj2 nfval_and_lam_lc.
